src/Init/Data/Slice/Operations.lean
@@ -28,15 +28,24 @@ and use `Std.Slice.iter` instead.
 def Internal.iter (s : Slice γ) [ToIterator s Id β] :=
   ToIterator.iter s
 
+class SliceSize (α : Type u) where
+  size (slice : Slice α) : Nat
+
+class LawfulSliceSize (α : Type u) [SliceSize α] [∀ s : Slice α, ToIterator s Id β]
+    [∀ s : Slice α, Iterator (ToIterator.State s Id) Id β] where
+  [finite : ∀ s : Slice α, Finite (ToIterator.State s Id) Id]
+  lawful :
+      letI (s : Slice α) : IteratorLoop (ToIterator.State s Id) Id Id := .defaultImplementation
+      ∀ s : Slice α, SliceSize.size s = (ToIterator.iter s).count
+
 /--
 Returns the number of elements with distinct indices in the given slice.
 
 Example: `#[1, 1, 1][0...2].size = 2`.
 -/
 @[always_inline, inline]
-def size (s : Slice γ) [ToIterator s Id β] [Iterator (ToIterator.State s Id) Id β]
-    [IteratorSize (ToIterator.State s Id) Id] :=
-  Internal.iter s |>.size
+def size (s : Slice γ) [SliceSize γ] :=
+  SliceSize.size s
 
 /-- Allocates a new array that contains the elements of the slice. -/
 @[always_inline, inline]
