src/Init/Data/Range/Polymorphic/NatLemmas.lean
@@ -28,40 +28,32 @@ theorem ClosedOpen.toList_succ_succ {m n : Nat} :
 @[simp]
 theorem size_Rcc {a b : Nat} :
     (a...=b).size = b + 1 - a := by
-  simp [Rcc.size, Std.Iterators.Iter.size, Std.Iterators.IteratorSize.size,
-    Rcc.Internal.iter, Std.Iterators.Iter.toIterM, Rxc.HasSize.size]
+  simp [Rcc.size, Rxc.HasSize.size]
 
 @[simp]
 theorem size_Rco {a b : Nat} :
     (a...b).size = b - a := by
-  simp only [Rco.size, Iterators.Iter.size, Iterators.IteratorSize.size, Iterators.Iter.toIterM,
-    Rco.Internal.iter, Rxo.HasSize.size, Rxc.HasSize.size, Id.run_pure]
+  simp only [Rco.size, Rxo.HasSize.size, Rxc.HasSize.size]
   omega
 
 @[simp]
 theorem size_Roc {a b : Nat} :
     (a<...=b).size = b - a := by
-  simp [Roc.size, Std.Iterators.Iter.size, Std.Iterators.IteratorSize.size,
-    Roc.Internal.iter, Std.Iterators.Iter.toIterM, Rxc.HasSize.size]
+  simp [Roc.size, Rxc.HasSize.size]
 
 @[simp]
 theorem size_Roo {a b : Nat} :
     (a<...b).size = b - a - 1 := by
-  simp only [Roo.size, Iterators.Iter.size, Iterators.IteratorSize.size, Iterators.Iter.toIterM,
-    Roo.Internal.iter, Rxo.HasSize.size, Rxc.HasSize.size, Id.run_pure]
-  omega
+  simp [Roo.size, Rxo.HasSize.size, Rxc.HasSize.size]
 
 @[simp]
 theorem size_Ric {b : Nat} :
     (*...=b).size = b + 1 := by
-  simp [Ric.size, Std.Iterators.Iter.size, Std.Iterators.IteratorSize.size,
-    Ric.Internal.iter, Std.Iterators.Iter.toIterM, Rxc.HasSize.size]
+  simp [Ric.size, Rxc.HasSize.size]
 
 @[simp]
 theorem size_Rio {b : Nat} :
     (*...b).size = b := by
-  simp only [Rio.size, Iterators.Iter.size, Iterators.IteratorSize.size, Iterators.Iter.toIterM,
-    Rio.Internal.iter, Rxo.HasSize.size, Rxc.HasSize.size, Id.run_pure]
-  omega
+  simp [Rio.size, Rxo.HasSize.size, Rxc.HasSize.size]
 
 end Std.PRange.Nat
