src/Std/Data/Iterators/Combinators/Monadic/Drop.lean
@@ -168,12 +168,4 @@ instance Drop.instIteratorLoopPartial {n : Type x → Type x'} [Monad m] [Monad 
     IteratorLoopPartial (Drop α m β) m n :=
   .defaultImplementation
 
-instance {α : Type w} [Monad Id] [Iterator α Id β] [Finite α Id] [IteratorLoop α Id Id] :
-    IteratorSize (Drop α Id β) Id :=
-  .defaultImplementation
-
-instance {α : Type w} [Monad Id] [Iterator α Id β] [IteratorLoopPartial α Id Id] :
-    IteratorSizePartial (Drop α Id β) Id :=
-  .defaultImplementation
-
 end Std.Iterators
