src/Std/Data/Iterators/Producers/Monadic/Array.lean
@@ -131,12 +131,4 @@ instance {α : Type w} [Monad m] {n : Type x → Type x'} [Monad n] :
     IteratorLoopPartial (ArrayIterator α) m n :=
   .defaultImplementation
 
-@[always_inline, inline]
-instance {α : Type w} : IteratorSize (ArrayIterator α) Id :=
-  .defaultImplementation
-
-@[always_inline, inline]
-instance {α : Type w} : IteratorSizePartial (ArrayIterator α) Id :=
-  .defaultImplementation
-
 end Std.Iterators
